pr/326/head/lf/terse/lean/LF.lean
@@ -10,3 +10,5 @@ import LF.IndProp
 import LF.Automation
 import LF.Typeclasses
 import LF.Postscript
+
+-- Built on 2026-09-04 18:43 UTC
